SyBloc/SBSemantics.v
@@ -24,17 +24,17 @@ Module Type SBSEMANTICS
        (Import Str     : STREAM              Op OpAux)
        (Import ExprSem : NLEXPRSEMANTICS Ids Op OpAux Clks ExprSyn Str).
 
-  Record mvalue :=
-    Mvalue { content_i: val;
-             reset_i: bool
-           }.
+  (* Record mvalue := *)
+  (*   Mvalue { content_i: val; *)
+  (*            reset_i: bool *)
+  (*          }. *)
 
   Record mvalues :=
     Mvalues { content: stream val;
               reset: stream bool
             }.
 
-  Definition memory := RMemory.memory mvalue.
+  (* Definition memory := RMemory.memory mvalue. *)
   Definition memories := RMemory.memory mvalues.
 
   Inductive reset_regs: stream bool -> memories -> Prop :=
@@ -62,6 +62,31 @@ Module Type SBSEMANTICS
                 /\ xs n = present (mvs.(content) n)
               end) ->
         mfby x v0 ls M xs.
+
+  Definition fby_eq (mems: PS.t) (eq: equation) : PS.t :=
+    match eq with
+    | EqFby x _ _ _ => PS.add x mems
+    | _ => mems
+    end.
+
+  Definition fbys (eqs: list equation) : PS.t :=
+    fold_left fby_eq eqs PS.empty.
+
+  Definition inst_eq (insts: PS.t) (eq: equation) : PS.t :=
+    match eq with
+    | EqReset _ _ i _ => PS.add i insts
+    | EqCall _ _ _ i _ => PS.add i insts
+    | _ => insts
+    end.
+
+  Definition insts (eqs: list equation) : PS.t :=
+    fold_left inst_eq eqs PS.empty.
+
+  Definition well_structured_memories (eqs: list equation) (M: memories) :=
+    (forall x,
+        find_val x M <> None <-> PS.In x (fbys eqs))
+    /\ forall x,
+      find_inst x M <> None <-> PS.In x (insts eqs).
 
   Section BlockSemantics.
 
@@ -104,6 +129,7 @@ Module Type SBSEMANTICS
                same_clock yss ->
                (forall n, absent_list (xss n) <-> absent_list (yss n)) ->
                Forall (sem_equation bk H M) bl.(b_eqs) ->
+               well_structured_memories bl.(b_eqs) M ->
                sem_block b M xss yss.
 
   End BlockSemantics.
@@ -153,6 +179,7 @@ Module Type SBSEMANTICS
         same_clock yss ->
         (forall n, absent_list (xss n) <-> absent_list (yss n)) ->
         Forall (sem_equation P bk H M) bl.(b_eqs) ->
+        well_structured_memories bl.(b_eqs) M ->
         Forall (P_equation bk H M) bl.(b_eqs) ->
         P_block b M xss yss.
 
@@ -168,6 +195,7 @@ Module Type SBSEMANTICS
       - destruct Sem; eauto.
       - destruct Sem.
         eapply BlockCase; eauto.
+        match goal with H: well_structured_memories _ _ |- _ => clear H end.
         match goal with H: Forall _ _ |- _ => induction H; auto end.
     Qed.
 
@@ -194,6 +222,147 @@ Module Type SBSEMANTICS
   Proof.
     intros ** Sem; split; inv Sem;
       assert_const_length xss; assert_const_length yss; auto.
+  Qed.
+
+  Lemma In_fold_left_fby_eq:
+    forall x eqs m,
+      PS.In x (fold_left fby_eq eqs m)
+      <-> PS.In x (fbys eqs) \/ PS.In x m.
+  Proof.
+    unfold fbys.
+    induction eqs as [|eq].
+    - split; auto.
+      destruct 1 as [H|].
+      apply not_In_empty in H; contradiction.
+      auto.
+    - split.
+      + intro H.
+        simpl; rewrite IHeqs.
+        simpl in H; apply IHeqs in H; destruct H; auto.
+        destruct eq; auto.
+        apply PS.add_spec in H.
+        destruct H.
+        rewrite H; left; right; apply PS.add_spec; intuition.
+        intuition.
+      + destruct 1 as [H|H].
+        * simpl in H; rewrite IHeqs in H; apply IHeqs; destruct H; auto.
+          right.
+          destruct eq; try (apply not_In_empty in H; contradiction).
+          simpl; apply PS.add_spec.
+          apply PS.add_spec in H; destruct H;
+            try apply not_In_empty in H; intuition.
+        * apply IHeqs; right; destruct eq; auto.
+          apply PS.add_spec; auto.
+  Qed.
+
+  Lemma In_fold_left_inst_eq:
+    forall x eqs m,
+      PS.In x (fold_left inst_eq eqs m)
+      <-> PS.In x (insts eqs) \/ PS.In x m.
+  Proof.
+    unfold insts.
+    induction eqs as [|eq].
+    - split; auto.
+      destruct 1 as [H|].
+      apply not_In_empty in H; contradiction.
+      auto.
+    - split.
+      + intro H.
+        simpl; rewrite IHeqs.
+        simpl in H; apply IHeqs in H; destruct H; auto.
+        destruct eq; auto; apply PS.add_spec in H; destruct H; auto;
+          rewrite H; left; right; apply PS.add_spec; auto.
+      + destruct 1 as [H|H].
+        * simpl in H; rewrite IHeqs in H; apply IHeqs; destruct H; auto.
+          right.
+          destruct eq; try (apply not_In_empty in H; contradiction);
+            simpl; apply PS.add_spec;
+              apply PS.add_spec in H; destruct H; auto;
+                apply not_In_empty in H; contradiction.
+        * apply IHeqs; right; destruct eq; auto;
+            apply PS.add_spec; auto.
+  Qed.
+
+  Lemma well_structured_def:
+    forall M x ck e eqs,
+      well_structured_memories (EqDef x ck e :: eqs) M <->
+      well_structured_memories eqs M.
+  Proof.
+    split; eauto.
+  Qed.
+
+  Lemma well_structured_add_inst_call:
+    forall M M' xs ck f i es eqs,
+      well_structured_memories eqs M ->
+      well_structured_memories (EqCall xs ck f i es :: eqs) (add_inst i M' M).
+  Proof.
+    intros ** WS.
+    constructor; unfold fbys, insts; simpl; split; intro H.
+    - rewrite find_val_add_inst in H; apply WS in H; auto.
+    - rewrite find_val_add_inst; apply WS in H; auto.
+    - rewrite In_fold_left_inst_eq.
+      destruct (ident_eqb x i) eqn: E;
+        [apply ident_eqb_eq in E; subst|apply ident_eqb_neq in E].
+      + right; apply PSE.MP.Dec.F.add_1; auto.
+      + rewrite find_inst_gso in H; auto.
+        apply WS in H; auto.
+    - destruct (ident_eqb x i) eqn: E;
+        [apply ident_eqb_eq in E; subst|apply ident_eqb_neq in E].
+      + rewrite find_inst_gss; intro; discriminate.
+      + rewrite find_inst_gso; auto.
+        apply WS.
+        apply In_fold_left_inst_eq in H as [|H]; auto.
+        apply PSE.MP.Dec.F.add_3 in H; auto.
+        contradict H; apply not_In_empty.
+  Qed.
+
+  Lemma well_structured_reset_call:
+    forall M xs ck f i es ck_r r eqs,
+      well_structured_memories (EqCall xs ck f i es :: eqs) M ->
+      well_structured_memories (EqReset ck_r f i r :: EqCall xs ck f i es :: eqs) M.
+  Proof.
+    inversion_clear 1 as [Vals Insts].
+    constructor; unfold fbys, insts in *; simpl in *.
+    - intro; rewrite Vals; reflexivity.
+    - intro; rewrite Insts.
+      rewrite 2 In_fold_left_inst_eq.
+      split; intros [H|H']; auto.
+      + rewrite PSE.MP.Dec.F.add_iff; auto.
+      + apply PSE.MP.Dec.F.add_iff in H' as []; auto.
+        rewrite PSE.MP.Dec.F.add_iff; auto.
+  Qed.
+
+  Corollary well_structured_add_inst_reset_call:
+    forall M M' xs ck f i es ck_r r eqs,
+      well_structured_memories eqs M ->
+      well_structured_memories (EqReset ck_r f i r :: EqCall xs ck f i es :: eqs) (add_inst i M' M).
+  Proof.
+    intros; apply well_structured_reset_call, well_structured_add_inst_call; auto.
+  Qed.
+
+  Lemma well_structured_add_val_fby:
+    forall M mvs x ck v0 e eqs,
+      well_structured_memories eqs M ->
+      well_structured_memories (EqFby x ck v0 e :: eqs) (add_val x mvs M).
+  Proof.
+    intros ** WS.
+    constructor; unfold fbys, insts; simpl; split; intro H.
+    - rewrite In_fold_left_fby_eq.
+      destruct (ident_eqb x x0) eqn: E;
+        [apply ident_eqb_eq in E; subst|apply ident_eqb_neq in E].
+      + right; apply PSE.MP.Dec.F.add_1; auto.
+      + rewrite find_val_gso in H; auto.
+        apply WS in H; auto.
+    - destruct (ident_eqb x x0) eqn: E;
+        [apply ident_eqb_eq in E; subst|apply ident_eqb_neq in E].
+      + rewrite find_val_gss; intro; discriminate.
+      + rewrite find_val_gso; auto.
+        apply WS.
+        apply In_fold_left_fby_eq in H as [|H]; auto.
+        apply PSE.MP.Dec.F.add_3 in H; auto.
+        contradict H; apply not_In_empty.
+    - rewrite find_inst_add_val in H; apply WS in H; auto.
+    - rewrite find_inst_add_val; apply WS in H; auto.
   Qed.
 
 End SBSEMANTICS.
