Common.v
@@ -2093,6 +2093,23 @@ Proof.
   - rewrite IHxs. rewrite PS.add_spec. intuition.
 Qed.
 
+Lemma in_fold_left_add:
+  forall x xs S,
+    PS.In x (fold_left (fun S' x => PS.add x S') xs S)
+    <->
+    In x xs \/ PS.In x S.
+Proof.
+  induction xs as [|y xs IH].
+  split; intro H; simpl in *;
+    intuition.
+  intro S; split; intro H.
+  - apply IH in H.
+    destruct H.
+    now left; constructor (assumption).
+    apply PS.add_spec in H; simpl; intuition.
+  - simpl; apply IH; simpl in H; intuition.
+Qed.
+
 (** types and clocks *)
 
 Section TypesAndClocks.
